WIP on shrinking goal size.

examples/QueryStructure/WeatherwDelegation.v
@@ -40,36 +40,42 @@ Definition WeatherSchema :=
     enforcing [attribute CELL_ID for MEASUREMENTS references CELLS].
 (* Try with three tables (distribution of areas per state) *)
 
+Definition Init := "Init".
+Definition AddCell := "AddCell".
+Definition AddMeasurement := "AddMeasurement".
+Definition CountCells := "CountCells".
+Definition LocalMax := "LocalMax".
+
 Definition WeatherSig : ADTSig :=
   ADTsignature {
-      Constructor "Init"           : unit                               -> rep,
-      (* Method "AddCell"        : rep x (WeatherSchema#CELLS)        -> rep x bool, *)
-      (*Method "AddMeasurement" : rep x (WeatherSchema#MEASUREMENTS) -> rep x bool, *)
-      Method "CountCells"     : rep x AreaCode                        -> rep x nat
-      (* Method "LocalMax"       : rep x (AreaCode * MeasurementType)    -> rep x option Z *)
+      Constructor Init           : unit                               -> rep,
+      Method AddCell        : rep x (WeatherSchema#CELLS)        -> rep x bool,
+      Method AddMeasurement : rep x (WeatherSchema#MEASUREMENTS) -> rep x bool,
+      Method CountCells     : rep x AreaCode                        -> rep x nat,
+      Method LocalMax       : rep x (AreaCode * MeasurementType)    -> rep x option Z
     }.
 
 Definition WeatherSpec : ADT WeatherSig :=
   QueryADTRep WeatherSchema {
-    Def Constructor "Init" (_ : unit) : rep := empty,
+    Def Constructor Init (_ : unit) : rep := empty,
 
-    (*update "AddCell" (cell : WeatherSchema#CELLS) : bool :=
-        Insert cell into CELLS, *)
+    update AddCell (cell : WeatherSchema#CELLS) : bool :=
+        Insert cell into CELLS,
 
-    (*update "AddMeasurement" (measurement : WeatherSchema#MEASUREMENTS) : bool :=
-        Insert measurement into MEASUREMENTS, *)
+    update AddMeasurement (measurement : WeatherSchema#MEASUREMENTS) : bool :=
+        Insert measurement into MEASUREMENTS,
 
-    query "CountCells" (area : AreaCode) : nat :=
+    query CountCells (area : AreaCode) : nat :=
       Count (For (cell in CELLS)
              Where (area = cell!AREA_CODE)
-             Return 1)
+             Return 1),
 
-     (* query "LocalMax" (params: AreaCode * MeasurementType) : option Z :=
+      query LocalMax (params: AreaCode * MeasurementType) : option Z :=
         MaxZ (For (cell in CELLS) (measurement in MEASUREMENTS)
               Where (cell!AREA_CODE = fst params)
               Where (measurement!MEASUREMENT_TYPE = snd params)
               Where (cell!CELL_ID = measurement!CELL_ID)
-              Return measurement!VALUE) *)
+              Return measurement!VALUE)
 }.
 
 Ltac CombineUse x y :=
@@ -79,21 +85,134 @@ Ltac CombineUse x y :=
       | _ => y a c
     end.
 
+Ltac foo :=
+  remove trivial insertion checks;
+    (* The trivial insertion checks involve the fresh id,
+       so we need to drill under the binder before
+       attempting to remove them. *)
+    rewrite refine_bind;
+    [ | reflexivity |
+      unfold pointwise_relation; intros; subst_strings;
+      repeat remove_trivial_insertion_constraints;
+      subst_strings;
+      (* These simplify and implement nontrivial constraint checks *)
+      repeat first
+             [ drop_symmetric_functional_dependencies
+             | fundepToQuery; try simplify with monad laws
+             | foreignToQuery; try simplify with monad laws
+             | setoid_rewrite refine_trivial_if_then_else; simplify with monad laws
+             ];
+             higher_order_reflexivity ];
+    finish honing.
+
+Ltac bar :=
+  simplify with monad laws;
+    subst_strings; repeat (setoid_rewrite DropQSConstraintsQuery_In; simpl);
+    repeat setoid_rewrite DropQSConstraintsQuery_In_UnderBinder;
+    simpl; pose_string_ids;
+    setoid_rewrite refineEquiv_pick_eq';
+    simplify with monad laws; cbv beta; simpl;
+    match goal with
+        H : DropQSConstraints_AbsR _ _ |- _ =>
+        unfold DropQSConstraints_AbsR in H; rewrite H
+    end;
+    finish honing.
+
+Definition WeatherSpec' : ADT WeatherSig.
+  let H := eval cbv delta [WeatherSpec
+                         QSGetNRelSchemaHeading GetNRelSchema
+                         GetNRelSchemaHeading Domain Specif.value
+                         IndexBound_tail IndexBound_head WeatherSpec] beta in WeatherSpec in
+      let H' := eval simpl in H in
+          exact H'.
+Defined.
+
+Definition SharpenedWeatherStation' :
+  sigT (fun adt => refineADT WeatherSpec' adt).
+Proof.
+  eexists.
+  Set Printing All.
+  Show Proof.
+  cbv beta delta [WeatherSpec' Specif.value].
+  pose_string_ids.
+  repeat match goal with
+               | |- context[BuildHeading ?attrlist] =>
+                 let heading := fresh "heading" in
+                 set (BuildHeading attrlist) as heading
+           end.
+  match goal with
+      |- context [@BuildADT (QueryStructure ?Rep) _ _ _ _] =>
+      eapply refineADT_BuildADT_Rep_refine_All with (AbsR := @DropQSConstraints_AbsR Rep);
+  [ repeat (first [eapply refine_Constructors_nil
+                        | eapply refine_Constructors_cons;
+                          [ intros;
+                            match goal with
+                              |  |- refine _ (?E _) => let H := fresh in set (H := E)
+                              | _ => idtac
+                            end | ] ])
+        | repeat (first [eapply refine_Methods_nil
+                        | eapply refine_Methods_cons;
+                          [ intros;
+                            match goal with
+                              |  |- refine _ (?E _ _) => let H := fresh in set (H := E)
+                              | _ => idtac
+                            end | ]
+                        ])]
+  end.
+  Show Proof.
+  apply Constructor_DropQSConstraints.
+  - subst heading; subst heading0; foo.
+  - foo.
+  - subst heading; subst heading0.
+    bar.
+  - subst heading; subst heading0; bar.
+Defined.
+
+
 Definition SharpenedWeatherStation :
   Sharpened WeatherSpec.
 Proof.
-  unfold WeatherSpec.
-
+  eapply SharpenStep.
+  eapply (projT2 SharpenedWeatherStation').
+  unfold SharpenedWeatherStation'; simpl.
   Start Profiling.
 
-  start honing QueryStructure.
   (* Old, explicit index selection*)
   (* make simple indexes using [[AREA_CODE]; [MEASUREMENT_TYPE; CELL_ID]]. *)
-  Show Profile.
 
-  make indexes using matchInclusionIndex.
+  GenerateIndexesForAll
+    ClauseMatchers
+    ltac:(fun attrlist =>
+            match goal with
+              | [ |- Sharpened (@BuildADT (UnConstrQueryStructure ?sch) _ _ _ _ )] =>
+                let sch' := eval simpl in (qschemaSchemas sch) in
+                    makeIndex' sch' attrlist
+                               ltac:(fun l =>
+                                       let index := fresh "Index" in
+                                       pose l as index;
+                                     revert Index;
+                                     pose_string_ids;
+                                     repeat match goal with
+                                              | |- context [ ``(?R) ] =>
+                                                let idx := fresh in
+                                                set ``(R) as fresh in *
+                                              | |- context [@Build_BoundedIndex ?A ?Bound ?idx ?bnd] =>
+                                                let idx := fresh in
+                                                set (@Build_BoundedIndex A Bound idx bnd) as idx in *
+                                            end;
+                                     repeat match goal with
+                                              | |- context[BuildHeading ?attrlist] =>
+                                                let heading := fresh "heading" in
+                                                set (BuildHeading attrlist) as heading
 
-  plan
+                                            end;
+                                     intros; cbv beta; simpl in *;
+                                       unfold Domain in *; simpl in *;
+                                       hone representation using (@DelegateToBag_AbsR sch index))
+            end).
+  - initializer.
+  - subst heading; subst heading0.
+    insertion
     ltac:(fun SC F indexed_attrs f k =>
             match goal with
               | _ => InclusionIndexUse SC F indexed_attrs f k
@@ -120,6 +239,240 @@ Proof.
                                           | _ => createLastInclusionTerm_dep dom f fds tail fs kind rest s k
                                           | _ => createLastRangeTerm_dep dom f fds tail fs kind rest s k
                                         end).
+  - subst heading; subst heading0.
+    insertion
+    ltac:(fun SC F indexed_attrs f k =>
+            match goal with
+              | _ => InclusionIndexUse SC F indexed_attrs f k
+              | _ => RangeIndexUse SC F indexed_attrs f k
+            end)
+           ltac:(fun f fds tail fs kind EarlyIndex LastIndex rest s k =>
+                   match goal with
+                     | _ => createEarlyInclusionTerm f fds tail fs kind EarlyIndex LastIndex rest s k
+                     | _ => createEarlyRangeTerm f fds tail fs kind EarlyIndex LastIndex rest s k
+                   end)
+                  ltac:(fun f fds tail fs kind s k =>
+                          match goal with
+                            | _ => createLastInclusionTerm f fds tail fs kind s k
+                            | _ => createLastRangeTerm f fds tail fs kind s k
+                          end)
+                         ltac:(fun SC F indexed_attrs visited_attrs f T k =>
+                                 match goal with
+                                   | _ => InclusionIndexUse_dep SC F indexed_attrs visited_attrs f T k
+                                   | _ => RangeIndexUse_dep SC F indexed_attrs visited_attrs f T k
+                                 end)
+                                randomCrab
+                                ltac:(fun dom f fds tail fs kind rest s k =>
+                                        match goal with
+                                          | _ => createLastInclusionTerm_dep dom f fds tail fs kind rest s k
+                                          | _ => createLastRangeTerm_dep dom f fds tail fs kind rest s k
+                                        end).
+  - observer
+    ltac:(fun SC F indexed_attrs f k =>
+            match goal with
+              | _ => InclusionIndexUse SC F indexed_attrs f k
+              | _ => RangeIndexUse SC F indexed_attrs f k
+            end)
+           ltac:(fun f fds tail fs kind EarlyIndex LastIndex rest s k =>
+                   match goal with
+                     | _ => createEarlyInclusionTerm f fds tail fs kind EarlyIndex LastIndex rest s k
+                     | _ => createEarlyRangeTerm f fds tail fs kind EarlyIndex LastIndex rest s k
+                   end)
+                  ltac:(fun f fds tail fs kind s k =>
+                          match goal with
+                            | _ => createLastInclusionTerm f fds tail fs kind s k
+                            | _ => createLastRangeTerm f fds tail fs kind s k
+                          end)
+                         ltac:(fun SC F indexed_attrs visited_attrs f T k =>
+                                 match goal with
+                                   | _ => InclusionIndexUse_dep SC F indexed_attrs visited_attrs f T k
+                                   | _ => RangeIndexUse_dep SC F indexed_attrs visited_attrs f T k
+                                 end)
+                                randomCrab
+                                ltac:(fun dom f fds tail fs kind rest s k =>
+                                        match goal with
+                                          | _ => createLastInclusionTerm_dep dom f fds tail fs kind rest s k
+                                          | _ => createLastRangeTerm_dep dom f fds tail fs kind rest s k
+                                        end).
+  - observer
+    ltac:(fun SC F indexed_attrs f k =>
+            match goal with
+              | _ => InclusionIndexUse SC F indexed_attrs f k
+              | _ => RangeIndexUse SC F indexed_attrs f k
+            end)
+           ltac:(fun f fds tail fs kind EarlyIndex LastIndex rest s k =>
+                   match goal with
+                     | _ => createEarlyInclusionTerm f fds tail fs kind EarlyIndex LastIndex rest s k
+                     | _ => createEarlyRangeTerm f fds tail fs kind EarlyIndex LastIndex rest s k
+                   end)
+                  ltac:(fun f fds tail fs kind s k =>
+                          match goal with
+                            | _ => createLastInclusionTerm f fds tail fs kind s k
+                            | _ => createLastRangeTerm f fds tail fs kind s k
+                          end)
+                         ltac:(fun SC F indexed_attrs visited_attrs f T k =>
+                                 match goal with
+                                   | _ => InclusionIndexUse_dep SC F indexed_attrs visited_attrs f T k
+                                   | _ => RangeIndexUse_dep SC F indexed_attrs visited_attrs f T k
+                                 end)
+                                randomCrab
+                                ltac:(fun dom f fds tail fs kind rest s k =>
+                                        match goal with
+                                          | _ => createLastInclusionTerm_dep dom f fds tail fs kind rest s k
+                                          | _ => createLastRangeTerm_dep dom f fds tail fs kind rest s k
+                                        end).
+    Unset Printing All.
+    idtac.
+    simpl.
+    Set Printing All.
+    idtac.
+    Unset Printing All.
+    pose_string_ids.
+    repeat match goal with
+             | |- context [ ``(?R) ] =>
+               let idx := fresh in
+               set ``(R) as fresh in *
+             | |- context [@Build_BoundedIndex ?A ?Bound ?idx ?bnd] =>
+               let idx := fresh in
+               set (@Build_BoundedIndex A Bound idx bnd) as idx in *
+           end;
+      repeat match goal with
+               | |- context[BuildHeading ?attrlist] =>
+                 let heading := fresh "heading" in
+                 set (BuildHeading attrlist) as heading
+                                                  
+             end.
+    Set Printing All.
+    idtac.
+    repeat match goal with
+        |- context[IndexedQueryStructure ?qs_schema ?search_terms] =>
+        let repType := fresh "repType" in
+        set (IndexedQueryStructure qs_schema search_terms) as repType in *
+    end.
+    Check CallBagMethod.
+    repeat match goal with
+               |- appcontext[@CallBagMethod ?qs_schema (@icons ?A ?B ?a ?As ?b ?Bs)] => 
+               let index := fresh "Index" in
+               set (@icons A B a As b Bs) as index in *
+           end.
+    Print SearchUpdateTerms.
+    repeat match goal with
+               |- context [@Build_SearchUpdateTerms
+                             ?heading ?stType ?stMatcher
+                             ?utType ?utApply] =>
+               let stu := fresh "SearchUpdateTerm" in
+               set (@Build_SearchUpdateTerms heading stType stMatcher utType utApply) as stu in *
+           end.
+    Unset Printing All.
+    idtac.
+  - simpl.
+
+
+    subst_strings; pose_string_ids.
+  Set Printing All.
+  idtac.
+  honeOne
+    ltac:(fun SC F indexed_attrs f k =>
+            match goal with
+              | _ => InclusionIndexUse SC F indexed_attrs f k
+              | _ => RangeIndexUse SC F indexed_attrs f k
+            end)
+           ltac:(fun f fds tail fs kind EarlyIndex LastIndex rest s k =>
+                   match goal with
+                     | _ => createEarlyInclusionTerm f fds tail fs kind EarlyIndex LastIndex rest s k
+                     | _ => createEarlyRangeTerm f fds tail fs kind EarlyIndex LastIndex rest s k
+                   end)
+                  ltac:(fun f fds tail fs kind s k =>
+                          match goal with
+                            | _ => createLastInclusionTerm f fds tail fs kind s k
+                            | _ => createLastRangeTerm f fds tail fs kind s k
+                          end)
+                         ltac:(fun SC F indexed_attrs visited_attrs f T k =>
+                                 match goal with
+                                   | _ => InclusionIndexUse_dep SC F indexed_attrs visited_attrs f T k
+                                   | _ => RangeIndexUse_dep SC F indexed_attrs visited_attrs f T k
+                                 end)
+                                randomCrab
+                                ltac:(fun dom f fds tail fs kind rest s k =>
+                                        match goal with
+                                          | _ => createLastInclusionTerm_dep dom f fds tail fs kind rest s k
+                                          | _ => createLastRangeTerm_dep dom f fds tail fs kind rest s k
+                                        end).
+  Set Printing All.
+  idtac.
+  simpl.
+  subst_strings; pose_string_ids.
+  subst heading; subst heading0.
+  repeat match goal with
+           | |- context[BuildHeading ?attrlist] =>
+             let heading := fresh "heading" in
+             set (BuildHeading attrlist) as heading
+         end.
+  honeOne
+    ltac:(fun SC F indexed_attrs f k =>
+            match goal with
+              | _ => InclusionIndexUse SC F indexed_attrs f k
+              | _ => RangeIndexUse SC F indexed_attrs f k
+            end)
+           ltac:(fun f fds tail fs kind EarlyIndex LastIndex rest s k =>
+                   match goal with
+                     | _ => createEarlyInclusionTerm f fds tail fs kind EarlyIndex LastIndex rest s k
+                     | _ => createEarlyRangeTerm f fds tail fs kind EarlyIndex LastIndex rest s k
+                   end)
+                  ltac:(fun f fds tail fs kind s k =>
+                          match goal with
+                            | _ => createLastInclusionTerm f fds tail fs kind s k
+                            | _ => createLastRangeTerm f fds tail fs kind s k
+                          end)
+                         ltac:(fun SC F indexed_attrs visited_attrs f T k =>
+                                 match goal with
+                                   | _ => InclusionIndexUse_dep SC F indexed_attrs visited_attrs f T k
+                                   | _ => RangeIndexUse_dep SC F indexed_attrs visited_attrs f T k
+                                 end)
+                                randomCrab
+                                ltac:(fun dom f fds tail fs kind rest s k =>
+                                        match goal with
+                                          | _ => createLastInclusionTerm_dep dom f fds tail fs kind rest s k
+                                          | _ => createLastRangeTerm_dep dom f fds tail fs kind rest s k
+                                        end).
+  simpl.
+  subst_strings; pose_string_ids.
+  repeat match goal with
+           | |- context[BuildHeading ?attrlist] =>
+             let heading := fresh "heading" in
+             set (BuildHeading attrlist) as heading
+         end.
+  Print IndexedQueryStructure.
+
+        Set Printing All.
+        honeOne
+    ltac:(fun SC F indexed_attrs f k =>
+            match goal with
+              | _ => InclusionIndexUse SC F indexed_attrs f k
+              | _ => RangeIndexUse SC F indexed_attrs f k
+            end)
+           ltac:(fun f fds tail fs kind EarlyIndex LastIndex rest s k =>
+                   match goal with
+                     | _ => createEarlyInclusionTerm f fds tail fs kind EarlyIndex LastIndex rest s k
+                     | _ => createEarlyRangeTerm f fds tail fs kind EarlyIndex LastIndex rest s k
+                   end)
+                  ltac:(fun f fds tail fs kind s k =>
+                          match goal with
+                            | _ => createLastInclusionTerm f fds tail fs kind s k
+                            | _ => createLastRangeTerm f fds tail fs kind s k
+                          end)
+                         ltac:(fun SC F indexed_attrs visited_attrs f T k =>
+                                 match goal with
+                                   | _ => InclusionIndexUse_dep SC F indexed_attrs visited_attrs f T k
+                                   | _ => RangeIndexUse_dep SC F indexed_attrs visited_attrs f T k
+                                 end)
+                                randomCrab
+                                ltac:(fun dom f fds tail fs kind rest s k =>
+                                        match goal with
+                                          | _ => createLastInclusionTerm_dep dom f fds tail fs kind rest s k
+                                          | _ => createLastRangeTerm_dep dom f fds tail fs kind rest s k
+                                        end).
+
   Show Profile.
   Time FullySharpenQueryStructure WeatherSchema Index.
   simplify with monad laws.
